ironfleet/src/Dafny/Distributed/Protocol/RSL/FailureProof/FailureHelpers.i.dfy
@@ -18,25 +18,30 @@ function {:opaque} TBEpoch1() : Timestamp
   0
 }
 
+function {:opaque} TBEpoch2() : Timestamp
+{
+  0
+}
+
 // TODO: move these to a different file
 function {:opaque} EpochQD(nextActionIndex:int) : Timestamp
 {
   0
 }
 
-function {:opaque} FirstEpochEnd(nextActionIndex:int) : Timestamp
+function {:opaque} FirstEpochEnd() : Timestamp
 {
   0
 }
 
-function {:opaque} SecondEpochEnd(nextActionIndex:int) : Timestamp
+function {:opaque} SecondEpochEnd() : Timestamp
 {
-  0
+  FirstEpochEnd() // + EpochLength() + TimeActionRange(0)
 }
 
 function {:opaque} TBFirstSuspectingHB() : Timestamp
 {
-  0
+  SecondEpochEnd() // + HBPeriod() + TimeActionRange(0)
 }
 
 lemma EpochQDHelper()
